Progress in typing_trm_subst

ML_SP_Definitions.v
@@ -830,7 +830,7 @@ Inductive typing (gc:gc_info) : qenv -> kenv -> env -> trm -> typ -> Prop :=
       env_ok Q K E ->
       proper_instance K ((None, nil) :: Ks) Us ->
       (forall R Xs, fresh L (1 + length Us) (R :: Xs) ->
-        [ qvar R :: Q; K & kinds_open_vars ((None, rvar_f R :: nil) :: Ks) Xs; E
+        [ Q; K & kinds_open_vars ((None, rvar_f R :: nil) :: Ks) Xs; E
         | gc_raise gc |= trm_open_rigid t (rvar_f R) ~: typ_open_vars T Xs ]) ->
       [ Q; K; E | gc |= trm_rigid t ~: typ_open T Us ]
   | typing_use : forall n Ks Us Q K E t T1 T2,
